prove Validity, along with all SLOC metrics

paxos/proof.dfy
@@ -15,10 +15,10 @@ predicate Validity(c:Constants, ds:DistrSys, v:Value)
     requires c.WF()
     requires ds.WF(c)
 {
-    AllProcessesProposeV(c, ds, v) ==> AllDecidedProcessesDecidesV(c, ds, v)
+    AllProcessesInitV(c, ds, v) ==> AllDecidedProcessesDecidesV(c, ds, v)
 }
 
-predicate AllProcessesProposeV(c:Constants, ds:DistrSys, v:Value) 
+predicate AllProcessesInitV(c:Constants, ds:DistrSys, v:Value) 
     requires c.WF()
     requires ds.WF(c)
 {
@@ -39,25 +39,54 @@ predicate Validity_Inv(c:Constants, ds:DistrSys, v:Value)
     && c.WF()
     && ds.WF(c)
     && Validity(c, ds, v)
+    && Validity_Inv_AllLdrProposeV(c, ds, v)
+    && Validity_Inv_AllAccAcceptsV(c, ds, v)
+    && Validity_Inv_AllMessegesContainV(c, ds, v)
+}
+
+predicate Validity_Inv_AllMessegesContainV(c:Constants, ds:DistrSys, v:Value) {
+    forall pkt | pkt in ds.network.sentPackets :: MessageContainsV(pkt.msg, v)
+}
+
+predicate MessageContainsV(m: Message, v:Value) {
+    match m {
+        case Prepare(bal) => true
+        case Promise(bal, val) => val != v ==> val == Nil
+        case Propose(bal, val) => val == v
+        case Accept(bal) =>  true
+        case Preempt(bal, val) => val != v ==> val == Nil
+    }
+}
+
+predicate Validity_Inv_AllAccAcceptsV(c:Constants, ds:DistrSys, v:Value) 
+    requires c.WF()
+    requires ds.WF(c)
+{
+    forall i | c.ValidAccIdx(i) :: ds.acceptors[i].accepted != v ==> ds.acceptors[i].accepted == Nil 
+}
+
+predicate Validity_Inv_AllLdrProposeV(c:Constants, ds:DistrSys, v:Value)
+    requires c.WF()
+    requires ds.WF(c)
+{
+    forall i | c.ValidLdrIdx(i) :: ds.leaders[i].val == v
 }
 
 
 /* Init ==>  Validity_Inv */
 lemma InitImpliesInv(c:Constants, ds:DistrSys, v:Value) 
     requires Init(c, ds)
+    requires AllProcessesInitV(c, ds, v)
     ensures Validity_Inv(c, ds, v)
 {}
+
 
 /* Validity_Inv && Next ==>  Validity_Inv' */
 lemma NextPreservesInv(c:Constants, v:Value, ds:DistrSys, ds':DistrSys) 
     requires Validity_Inv(c, ds, v)
+    requires AllProcessesInitV(c, ds, v)
     requires Next(c, ds, ds')
     ensures Validity_Inv(c, ds', v)
-{
-    // TODO
-    assume false;
-}
-
-
+{}
 
 }
